heap_lang/notation.v
@@ -14,22 +14,28 @@ Coercion of_val : val >-> expr.
 
 (** Syntax inspired by Coq/Ocaml. Constructions with higher precedence come
     first. *)
+(* We have overlapping notation for values and expressions, with the expressions
+   coming first. This way, parsing as a value will be preferred. If an expression
+   was needed, the coercion of_val will be called. *)
 (* What about Arguments for hoare triples?. *)
+Notation "' l" := (Lit l) (at level 8, format "' l") : lang_scope.
 Notation "' l" := (LitV l) (at level 8, format "' l") : lang_scope.
 Notation "! e" := (Load e%L) (at level 10, format "! e") : lang_scope.
 Notation "'ref' e" := (Alloc e%L) (at level 30) : lang_scope.
+Notation "- e" := (UnOp MinusUnOp e%L) (at level 35, right associativity) : lang_scope.
 Notation "e1 + e2" := (BinOp PlusOp e1%L e2%L)
   (at level 50, left associativity) : lang_scope.
 Notation "e1 - e2" := (BinOp MinusOp e1%L e2%L)
   (at level 50, left associativity) : lang_scope.
-Notation "- e" := (UnOp MinusUnOp e%L) (at level 35, right associativity) : lang_scope.
-Notation "~ e" := (UnOp NegOp e%L) (at level 75, right associativity) : lang_scope.
 Notation "e1 ≤ e2" := (BinOp LeOp e1%L e2%L) (at level 70) : lang_scope.
 Notation "e1 < e2" := (BinOp LtOp e1%L e2%L) (at level 70) : lang_scope.
 Notation "e1 = e2" := (BinOp EqOp e1%L e2%L) (at level 70) : lang_scope.
+Notation "~ e" := (UnOp NegOp e%L) (at level 75, right associativity) : lang_scope.
 (* The unicode ← is already part of the notation "_ ← _; _" for bind. *)
 Notation "e1 <- e2" := (Store e1%L e2%L) (at level 80) : lang_scope.
 Notation "'rec:' f x := e" := (Rec f x e%L)
+  (at level 102, f at level 1, x at level 1, e at level 200) : lang_scope.
+Notation "'rec:' f x := e" := (RecV f x e%L)
   (at level 102, f at level 1, x at level 1, e at level 200) : lang_scope.
 Notation "'if' e1 'then' e2 'else' e3" := (If e1%L e2%L e3%L)
   (at level 200, e1, e2, e3 at level 200) : lang_scope.
@@ -39,6 +45,8 @@ are stated explicitly instead of relying on the Notations Let and Seq as
 defined above. This is needed because App is now a coercion, and these
 notations are otherwise not pretty printed back accordingly. *)
 Notation "λ: x , e" := (Lam x e%L)
+  (at level 102, x at level 1, e at level 200) : lang_scope.
+Notation "λ: x , e" := (LamV x e%L)
   (at level 102, x at level 1, e at level 200) : lang_scope.
 Notation "'let:' x := e1 'in' e2" := (Lam x e2%L e1%L)
   (at level 102, x at level 1, e1, e2 at level 200) : lang_scope.
